ClickMG.v
@@ -73,7 +73,6 @@ Section TokenMG.
   stage has received a token or not on reset, and whether the current stage
   generates a token or not on reset. *)
 
-Print marked_graph.
 
   Definition init_marking_flag (in_flag : token_flag) (out_flag : token_flag) 
       : forall t1 t2, stage_place t1 t2 -> nat :=
@@ -121,26 +120,54 @@ Print marked_graph.
 End TokenMG.
 
 Existing Instance token_transition_eq_dec.
+Arguments MG_SS {name name_dec transition transition_dec} MG {MG_scheme}.
 
-Section SS_to_TokenMG.
+Section TokenMG_to_SS.
 
   Variable even odd : Set.
-  Context `{naming_scheme name even odd}.
+
+  Class stage_naming_scheme `{naming_scheme name even odd} :=
+    {stage_place_name : forall {t1 t2 : token_transition}, stage_place t1 t2 -> name}.
+
+  Context `{scheme : naming_scheme name even odd}.
+  Context `{x_scheme : stage_naming_scheme}.
+  Definition name_is_stage_place_dec : forall x,
+                           {t1 : token_transition &
+                           {t2 : token_transition & {p : stage_place t1 t2 & x = stage_place_name p}}}
+                        + {forall t1 t2 (p : stage_place t1 t2), x <> stage_place_name p}.
+  Proof.
+    intros x.
+
+    Ltac compare_place_name x p :=
+      compare x (stage_place_name p);
+        [ left; do 3 eexists; reflexivity | ].
+    compare_place_name x left_ack_left_req.
+    compare_place_name x clk_fall_left_req.
+    compare_place_name x right_req_left_req.
+    compare_place_name x clk_rise_left_ack.
+    compare_place_name x clk_rise_right_req.
+    compare_place_name x right_req_right_ack.
+    compare_place_name x clk_fall_right_ack.
+    compare_place_name x left_ack_right_ack.
+    compare_place_name x clock_fall.
+    compare_place_name x left_req_clk_rise.
+    compare_place_name x right_ack_clk_rise.
+    right. intros t1 t2 p; destruct p; auto.
+  Defined.
+
   Variable dp_reset_n ctrl_reset_n : name.
 
   Variable l : latch even odd.
   Variable in_flag : token_flag.
-  Definition out_flag := latch_to_token_flag l.
-      
+  Let out_flag := latch_to_token_flag l.
 
-
-  Definition transition_update_value (t : token_transition) (v : value) : value :=
+  Definition token_transition_update_value (t : token_transition) (v : value) : value :=
     match t with
     | clk_rise => Bit1
     | clk_fall => Bit0
     | _ => neg_value v
     end.
-  Definition transition_name (t : token_transition) : name :=
+  Definition token_transition_name (t : token_transition) : name :=
     match t with
     | left_ack => ack (latch_input l)
     | left_req => req (latch_input l)
@@ -149,8 +176,222 @@ Section SS_to_TokenMG.
     | clk_rise  => latch_clk l
     | clk_fall  => latch_clk l
     end.
-    
 
+  Program Instance stage_MG_scheme : MG_naming_scheme name (stage_MG in_flag out_flag) :=
+  {| transition_name := token_transition_name
+   ; place_name := @stage_place_name _ _
+   ; name_is_place_dec := name_is_stage_place_dec
+   ; transition_update_value := token_transition_update_value
+   ; input_transition := from_list [left_req; right_ack]
+   |}.
+
+  Definition stage_MG_SS : StateSpace name := MG_SS (stage_MG in_flag out_flag).
+
+
+End TokenMG_to_SS.
+
+Arguments name_is_place_dec {name transition} MG {MG_naming_scheme}.
+Existing Instance stage_MG_scheme.
+About stage_MG_scheme.
+Arguments traces_of {name}.
+Arguments stage_MG_SS {even odd} {scheme x_scheme} : rename.
+
+Section SS_to_TokenMG.
+
+  Variable even odd : Set.
+  Context `{scheme : naming_scheme name even odd}.
+  Context `{x_scheme : stage_naming_scheme even odd}.
+
+
+  Variable l : latch even odd.
+  Let out_flag := latch_to_token_flag l.
+  (* in_flag is opposite of out_flag here *)
+  Let in_flag := match l with
+                 | Odd _ => Token
+                 | Even _ => NonToken
+                 end.
+
+  Definition init_stage_MG_state : state name.
+  Proof.
+    intros x.
+    destruct (name_is_place_dec (stage_MG in_flag out_flag) x)
+      as [[t1 [t2 [p x_is_p]]] | x_not_p]; [ | exact (σR l x)].
+    (* here, x = stage_place_name p, so the value should be the value in the initial marking *)
+    exact (Num (init_marking (stage_MG in_flag out_flag) _ _ p)).
+  Defined.
+
+  (* The theorem *)
+  Theorem MG_refines_stage :
+    traces_of (latch_stage l) (σR l) ⊆ traces_of (stage_MG_SS l in_flag) init_stage_MG_state.
+  Proof.
+    unfold traces_of.
+    intros t Hstage.
+    destruct Hstage as [τ Hstage].
+    (* Need to define a relation between <t,τ> acceepted by (latch_stage l) and
+    <t,τ'> accepted by (stage_MG_SS l in_flag), and then prove that whenever
+    latch_stage l ⊢ σR l →*{t} τ, there exists a τ' such that
+    latch_stage l ⊢ init_stage_MG_state →*{t} τ'. *)
+  Abort.
+
+Print event.
+(*
+  Lemma left_req_inversion :
+    latch_stage l ⊢ σR l →{Some (Event (
+
+*)
+
+
+  Notation "σ1 'R{' t '}' σ2" := (relate_trace name (latch_stage l) (stage_MG_SS l in_flag)
+                      (σR l) init_stage_MG_state
+                      σ1 t σ2)
+    (left associativity, at level 92).
+
+
+  Definition latch_clk_component := clk_component (latch_input l) (latch_output l)
+                                      ctrl_reset_n (latch_clk l) (latch_state0 l)
+                                      (latch_to_token_flag l).
+  
+
+  Lemma left_req_inversion : forall σ σ' v,
+    latch_stage l ⊢ σ →{Some (Event (req (latch_input l)) v)} Some σ' ->
+    stable latch_clk_component σ 
+    /\ v = neg_value (σ (req (latch_input l))).
+  Proof.
+    intros.
+    unfold latch_clk_component, clk_component.
+    split.
+    apply func_stable_equiv.
+    * admit (* true *).
+    * admit (* true *).
+    * admit (* needs work *).
+  Admitted.
+  Lemma right_ack_inversion : forall σ σ' v,
+    latch_stage l ⊢ σ →{Some (Event (ack (latch_output l)) v)} Some σ' ->
+    stable latch_clk_component σ.
+  Admitted.
+  Definition latch_left_ack_component :=
+    ack_i_output (latch_input l) (latch_state0 l) (latch_to_token_flag l).
+  Lemma left_ack_inversion : forall σ σ' v,
+    latch_stage l ⊢ σ →{Some (Event (ack (latch_input l)) v)} Some σ' ->
+    ~ stable latch_left_ack_component σ.
+  Admitted.
+  Lemma right_req_inversion : forall σ σ' v,
+    latch_stage l ⊢ σ →{Some (Event (req (latch_output l)) v)} Some σ' ->
+    σ (req (latch_output l)) <> σ (latch_state0 l).
+  Admitted.
+  Lemma clk_inversion : forall σ σ' v,
+    latch_stage l ⊢ σ →{Some (Event (latch_clk l) v)} Some σ' ->
+       σ (latch_clk l) = σ (latch_old_clk l)
+    /\ ~ stable latch_clk_component σ.
+  Admitted.
+
+
+  Lemma left_req_relation_enabled : forall σ1 t σ2,
+    σ1 R{t} σ2 ->
+    stable latch_clk_component σ1 ->
+    is_enabled (stage_MG in_flag out_flag) left_req (state_to_marking σ2).
+  Admitted.
+  Lemma right_ack_relation_enabled : forall σ1 t σ2,
+    σ1 R{t} σ2 ->
+    stable latch_clk_component σ1 ->
+    is_enabled (stage_MG in_flag out_flag) right_ack (state_to_marking σ2).
+  Admitted.
+  Lemma left_ack_relation_enabled : forall σ1 t σ2,
+    σ1 R{t} σ2 ->
+    ~ stable latch_left_ack_component σ1 ->
+    is_enabled (stage_MG in_flag out_flag) left_ack (state_to_marking σ2).
+  Admitted.
+  Lemma right_req_relation_enabled : forall σ1 t σ2,
+    σ1 R{t} σ2 ->
+    σ1 (req (latch_output l)) <> σ1 (latch_state0 l) ->
+    is_enabled (stage_MG in_flag out_flag) right_req (state_to_marking σ2).
+  Admitted.
+
+  (* This isn't quite right... *)
+  Lemma clk_rise_relation_enabled : forall σ1 t σ2,
+    σ1 R{t} σ2 ->
+    σ1 (latch_clk l) = σ1 (latch_old_clk l) ->
+    σ1 (latch_clk l) = Bit0 ->
+    ~ stable latch_clk_component σ1 ->
+    is_enabled (stage_MG in_flag out_flag) clk_rise (state_to_marking σ2).
+  Admitted.
+  Lemma clk_fall_relation_enabled : forall σ1 t σ2,
+    σ1 R{t} σ2 ->
+    σ1 (latch_clk l) = σ1 (latch_old_clk l) ->
+    σ1 (latch_clk l) = Bit1 ->
+    ~ stable latch_clk_component σ1 ->
+    is_enabled (stage_MG in_flag out_flag) clk_fall (state_to_marking σ2).
+  Admitted.
+  
+
+
+  Definition visible_domain (S : StateSpace name) := space_input S ∪ space_output S.
+  (* Note: this will only be true for "well-formed" state space relations *)
+  Lemma step_visible : forall S σ x v σ',
+    S ⊢ σ →{Some (Event x v)} Some σ' ->
+    x ∈ visible_domain S.
+  Admitted.
+
+
+  Hypothesis dom_all_disjoint :
+    all_disjoint
+       [req (latch_input l); ack (latch_input l); req (latch_output l); ack (latch_output l); ctrl_reset_n;
+       dp_reset_n; latch_hidden l; latch_clk l; latch_old_clk l; latch_state0 l; 
+       latch_not_state0 l].
+
+  Lemma MG_relate_trace_step_lemma :
+    relate_trace_step_lemma name (latch_stage l) (stage_MG_SS l in_flag) (σR l) init_stage_MG_state.
+  Proof.
+    unfold relate_trace_step_lemma.
+    intros σ1 σ1' σ2 [x v] t Hstep Hrelate.
+    assert (Hx : x ∈ visible_domain (latch_stage l)).
+    { eapply step_visible; eauto. }
+    assert (Hx' : x ∈ from_list [req (latch_input l);ack (latch_input l);
+                                 ack (latch_output l);req (latch_output l);
+                                 latch_clk l]).
+    { unfold visible_domain in Hx.
+      destruct Hx as [? Hx | ? Hx].
+      * apply stage_input in Hx; auto.
+        decompose_set_structure; simpl; solve_set.
+      * apply stage_output in Hx; auto.
+        decompose_set_structure; simpl; solve_set.
+    }
+
+    clear Hx.
+    rename Hx' into Hx.
+    simpl in Hx.
+
+    decompose_set_structure.
+    + (* x = req (latch_input l) *)
+      apply left_req_inversion in Hstep.
+      destruct Hstep as [Hstable Hv].
+      assert (Henabled : is_enabled (stage_MG in_flag out_flag) left_req (state_to_marking σ2)).
+      { eapply left_req_relation_enabled; eauto. }
+      exists (update (fire_in_state left_req σ2) (req (latch_input l)) v).
+      apply transition_enabled with (t := left_req); auto.
+      { simpl.
+        replace (σ2 (req (latch_input l))) with (σ1 (req (latch_input l))); auto.
+        eapply relate_trace_domain; [ auto | | apply Hrelate | |].
+        { intros y Hy1 Hy2.
+          admit (* need to prove, but true *).
+        }
+        { unfold space_domain. simpl.
+          left. left. left. constructor. 2:{ solve_set. }
+          left. constructor. 2:{ solve_set. }
+          left. constructor. 2:{ unfold ack_i_output. admit (* true! *). }
+          solve_set.
+        }
+        { unfold space_domain. simpl. 
+          left. left.
+          exists left_req. split.
+          + solve_set.
+          + auto.
+        }
+      }
+    + (* x = ack (latch_input l) *)
+  Admitted.
+    
+(*
   Definition transition_to_event (t : token_transition) (σ : state name) : event name value :=
     let x := transition_name t in
     Event x (transition_update_value t (σ x)).
@@ -336,12 +577,10 @@ Admitted.
       destruct IHHstep as [m [t' [Hequiv HMG]]].
       exists m. exists t'. split; auto.
   Admitted.
+*)
         
 
   End SS_to_TokenMG.
 
 
-  Section Composition.
-
-  End Composition.
 End ClickMG.
