ClickRefinement.v
@@ -9,6 +9,7 @@ Open Scope list_scope.
 
 Require Import MarkedGraph.
 Require Import Click.
+Require Import ClickMG.
 
 Import EnsembleNotation.
 Open Scope ensemble_scope.
@@ -16,7 +17,71 @@ Require Import Coq.Program.Equality.
 
 Section MG_to_SS.
 
-  Print Marked
+  Print marked_graph.
+  Variable name : Set.
+  Context `{name_dec : eq_dec name}.
+
+  Variable transition : Set.
+  Context `{transition_dec : eq_dec transition}.
+  Variable MG : marked_graph transition.
+
+  Variable transition_name : transition -> name.
+  Variable place_name : forall t1 t2, place MG t1 t2 -> name.
+
+  Definition places_set : Ensemble name :=
+    fun x => exists t1 t2 (p : place MG t1 t2), x = place_name _ _ p.
+  Definition state_to_marking (σ : state name) : marking MG :=
+    fun t1 t2 p => val_to_nat (σ (place_name _ _ p)).
+
+  Hypothesis name_is_place_dec : forall x,
+                           {t1 : transition & {t2 : transition
+                                            & {p : place MG t1 t2 & x = place_name _ _ p}}}
+                         + {forall t1 t2 (p : place MG t1 t2), x <> place_name _ _ p}.
+
+  Definition fire_in_state (t : transition) (σ : state name) : state name :=
+    fun x =>
+    match name_is_place_dec x with
+    (* if x is not a place, do nothign *)
+    | inright _ => σ x
+    | inleft (existT _ tin (existT _ tout (existT _ p x_is_p))) =>
+      (* corner case: do nothing *)
+      if tin =? tout then σ x
+      (* if x is a place leading into t, increment the value *)
+      else if t =? tout then dec_value (σ x)
+      (* if x is a place leading out of t, decrement the value *)
+      else if t =? tin then inc_value (σ x)
+      (* otherwise do nothing *)
+      else σ x
+    end.
+
+  Variable transition_update_value : transition -> value -> value.
+  (* Condition: input_transition, output_transition should partition the set of all transitions *)
+  Variable input_transition : Ensemble transition.
+  Variable output_transition : Ensemble transition.
+
+  Inductive MG_SS_step
+    : state name -> option (event name value) -> option (state name) -> Prop :=
+
+  | transition_enabled σ σ' x v (t : transition) :
+    x = transition_name t ->
+    is_enabled MG t (state_to_marking σ) ->
+    v = transition_update_value t (σ x) ->
+    σ' = update (fire_in_state t σ) x v ->
+    MG_SS_step σ (Some (Event x v)) (Some σ')
+
+  | input_not_enabled σ x v t :
+    x = transition_name t ->
+    t ∈ input_transition ->
+    ~ is_enabled MG t (state_to_marking σ) ->
+   MG_SS_step σ (Some (Event x v)) None
+  .
+
+  Definition MG_SS : StateSpace name :=
+  {| space_input := fmap transition_name input_transition
+   ; space_output := fmap transition_name output_transition
+   ; space_internal := places_set
+   ; space_step := MG_SS_step
+   |}.
 
 End MG_to_SS.
 
@@ -32,7 +97,6 @@ Variable l : latch even odd.
 (** Define a state space [latch_stage_refinement such that every trace accepted
 by [latch_stage l] is also accepted by [latch_stage_refinement l] *)
 
-Print StateSpace. Print naming_scheme.
 Require Import ClickMG. 
 Class extended_naming_scheme :=
     {place_name : forall {t1 t2 : token_transition}, stage_place t1 t2 -> name}.
